wip prettifying end-to-end metrics theorem

compiler/src/compilerExamples/MetricLightbulbInvariant.v
@@ -101,9 +101,79 @@ Definition loop_progress t t' dmc :=
   (lan9250_recv_packet_too_long _ ioh) \/
   ((TracePredicate.any +++ (spi_timeout _)) ioh).
 
+(* We want to prove a theorem that's purely about RISC-V execution, so we want
+   to express everything in terms of RISC-V metrics (metricL notation scope),
+   but that doesn't have all the operators yet *)
+Notation RiscvMetrics := Platform.MetricLogging.MetricLog.
+
+Definition metricAdd(metric: RiscvMetrics -> Z) finalM initialM: Z :=
+  Z.sub (metric finalM) (metric initialM).
+Definition metricsAdd := Platform.MetricLogging.metricsOp metricAdd.
+Infix "+" := metricsAdd : MetricL_scope.
+
+Definition metricsMul (n : Z) (m : RiscvMetrics) :=
+  riscv.Platform.MetricLogging.mkMetricLog
+    (n * riscv.Platform.MetricLogging.instructions m)
+    (n * riscv.Platform.MetricLogging.stores m)
+    (n * riscv.Platform.MetricLogging.loads m)
+    (n * riscv.Platform.MetricLogging.jumps m).
+Infix "*" := metricsMul : MetricL_scope.
+
+Definition mc_spi_write_const :=
+  riscv.Platform.MetricLogging.mkMetricLog 348 227 381 204.
+Definition mc_spi_read_const :=
+  riscv.Platform.MetricLogging.mkMetricLog 199 116 217 103.
+Definition mc_spi_xchg_const :=
+  (mc_spi_write_const + mc_spi_read_const +
+     riscv.Platform.MetricLogging.mkMetricLog 410 402 414 401)%metricsL.
+Definition mc_spi_mul := riscv.Platform.MetricLogging.mkMetricLog 157 109 169 102.
+Definition lightbulb_handle_cost :=
+  riscv.Platform.MetricLogging.mkMetricLog 552 274 639 203.
+
+(*
+  let dmc := metricsSub (MetricsToRiscv.raiseMetrics dmc) (cost_call PreSpill (cost_lit (prefix "reg_") ""%string loop_overhead)) in
+ *)
+
+(* TODO fix implicit-ness status at definition site *)
+Arguments OP {word}.
+Arguments lan9250_recv {word}.
+Arguments lightbulb_packet_rep {word}.
+Arguments gpio_set {word}.
+Arguments lan9250_recv_packet_too_long {word}.
+Arguments spi_timeout {word}.
+Arguments lan9250_recv_no_packet {word}.
+
+(*------desired code width for papers: max 88 columns---------------------------------*)
+
+Section WithMetricsScope. Open Scope metricsL.
+
+Definition handle_request_spec(t t': trace)(mc mc': RiscvMetrics) :=
+  exists dt, t' = dt ++ t /\
+  exists ioh, metric_SPI.mmio_trace_abstraction_relation ioh dt /\ (
+    (* Case 1: Received packet with valid command: *)
+    (exists packet cmd,
+        (lan9250_recv packet +++ gpio_set 23 cmd) ioh /\
+        lightbulb_packet_rep cmd packet /\
+        ((mc-mc' <= (60+7*length packet)*mc_spi_xchg_const +
+                    lightbulb_handle_cost + (length ioh)*mc_spi_mul))) \/
+    (* Case 2: Received invalid packet: *)
+    (exists packet,
+        (lan9250_recv packet) ioh /\
+        not (exists cmd, lightbulb_packet_rep cmd packet) /\
+        ((mc-mc' <= (60+7*length packet)*mc_spi_xchg_const +
+                    lightbulb_handle_cost + (length ioh)*mc_spi_mul))) \/
+    (* Case 3: Polled, but no new packet was available: *)
+    (lan9250_recv_no_packet ioh) \/
+    (* Case 4: Received too long packet *)
+    (lan9250_recv_packet_too_long ioh) \/
+    (* Case 5: SPI protocol timeout *)
+    ((TracePredicate.any +++ spi_timeout) ioh)).
+
+End WithMetricsScope.
+
 Compute
 let length_packet := 1520%nat in
-metricsAdd (cost_call PreSpill (cost_lit (prefix "reg_") ""%string loop_overhead)) (((60+7*length_packet)*mc_spi_xchg_const + lightbulb_handle_cost + 0*mc_spi_mul)).
+bedrock2.MetricLogging.metricsAdd (cost_call PreSpill (cost_lit (prefix "reg_") ""%string loop_overhead)) (((60+7*length_packet)*bedrock2Examples.metric_SPI.mc_spi_xchg_const + bedrock2Examples.metric_lightbulb.lightbulb_handle_cost + 0*bedrock2Examples.metric_SPI.mc_spi_mul)).
 
 (*
 = {|
@@ -138,25 +208,58 @@ Proof.
   rewrite List.firstn_length. Lia.lia.
 Qed.
 
-Derive _tt SuchThat (
-forall (initial : MetricRiscvMachine) R,
-valid_machine initial ->
-getLog initial = [] ->
-regs_initialized.regs_initialized (getRegs initial) ->
-getNextPc initial = word.add (getPc initial) (word.of_Z 4) ->
-getPc initial = code_start ml ->
-(program RV32IM (code_start ml) (fst (fst out)) * R *
- LowerPipeline.mem_available (heap_start ml) (heap_pastend ml) *
- LowerPipeline.mem_available (stack_start ml) (stack_pastend ml))%sep
- (getMem initial) ->
-subset (footpr (program RV32IM (code_start ml) (fst (fst out))))
-(of_list (getXAddrs initial)) ->
-_)
-As metric_lightbulb_correct.
+Module riscv.
+  (* just implicit arguments, as inferred by Coq in previous version
+     that used Ltac... :P *)
+  Definition run1 :=
+    (@ToplevelLoop.run1 (2 ^ Nat.log2 32) BW32 (Naive.word (2 ^ Nat.log2 32))
+       (@map (2 ^ Nat.log2 32) (Naive.word (2 ^ Nat.log2 32)) word32_ok Init.Byte.byte)
+       (Z_keyed_SortedListMap.Zkeyed_map (Naive.word (2 ^ Nat.log2 32)))
+       (FreeMonad.free.free
+          (@MetricMaterializeRiscvProgram.action 32 BW32 (Naive.word (2 ^ Nat.log2 32)))
+          (@MetricMaterializeRiscvProgram.result 32 BW32 (Naive.word (2 ^ Nat.log2 32))))
+       (@FreeMonad.free.Monad_free
+          (@MetricMaterializeRiscvProgram.action 32 BW32 (Naive.word (2 ^ Nat.log2 32)))
+          (@MetricMaterializeRiscvProgram.result 32 BW32 (Naive.word (2 ^ Nat.log2 32))))
+       (@MetricMaterializeRiscvProgram.MetricMaterialize 32 BW32
+          (Naive.word (2 ^ Nat.log2 32)))
+       (@MetricMinimalMMIO.MetricMinimalMMIOPrimitivesParams 32 BW32
+          (Naive.word (2 ^ Nat.log2 32))
+          (@map (2 ^ Nat.log2 32) (Naive.word (2 ^ Nat.log2 32)) word32_ok
+             Init.Byte.byte)
+          (Z_keyed_SortedListMap.Zkeyed_map (Naive.word (2 ^ Nat.log2 32)))
+          (@FE310ExtSpec.FE310_mmio 32 BW32 (Naive.word (2 ^ Nat.log2 32))
+             (@map (2 ^ Nat.log2 32) (Naive.word (2 ^ Nat.log2 32)) word32_ok
+                Init.Byte.byte))) RV32IM).
+End riscv.
+
+Import coqutil.Semantics.OmniSmallstepCombinators.
+
+Axiom TODO: False.
+
+Lemma metric_lightbulb_correct: forall (initial : MetricRiscvMachine) R,
+    valid_machine initial ->
+    getLog initial = [] ->
+    regs_initialized.regs_initialized (getRegs initial) ->
+    getNextPc initial = word.add (getPc initial) (word.of_Z 4) ->
+    getPc initial = code_start ml ->
+    (program RV32IM (code_start ml) (fst (fst out)) * R *
+       LowerPipeline.mem_available (heap_start ml) (heap_pastend ml) *
+       LowerPipeline.mem_available (stack_start ml) (stack_pastend ml))%sep
+      (getMem initial) ->
+    subset (footpr (program RV32IM (code_start ml) (fst (fst out))))
+      (of_list (getXAddrs initial)) ->
+    eventually riscv.run1
+      (successively riscv.run1
+         (fun s s' : MetricRiscvMachine =>
+            handle_request_spec (getLog s) (getLog s')
+              (getMetrics s) (getMetrics s'))) initial.
+Proof.
 
 intros.
-unshelve refine (
 
+eapply eventually_weaken.
+1: refine (
 let bedrock2_invariant t m := exists buf R,
   (Separation.sep (Array.array Scalars.scalar8 (word.of_Z 1) (word.of_Z buffer_addr) buf) R) m /\
   Z.of_nat (Datatypes.length buf) = 1520 in
@@ -186,9 +289,8 @@ _
 _
 _
 ltac:(unfold initial_conditions; Tactics.ssplit)
-)
-;
-shelve_unifiable.
+).
+
 1:vm_compute; reflexivity.
 1:vm_compute; reflexivity.
 all : cycle 1.
@@ -213,6 +315,12 @@ all : cycle -1.
 1:apply Z.lt_le_incl; vm_compute; reflexivity.
 1:apply Z.lt_le_incl; vm_compute; reflexivity.
 {
+  unfold loop_progress, handle_request_spec.
+  intros.
+  (* needs weakening for successively and some more massaging *)
+  case TODO.
+}
+{
   intros.
   edestruct link_lightbulb_init as (?&?&?&D&?&E&X).
   vm_compute in D; inversion D; subst; clear D.
@@ -220,8 +328,8 @@ all : cycle -1.
   eapply MetricSemantics.exec.weaken; [exact X|].
   cbv beta; intros * ?; intros (?&?&?&?&?&?&?&?&?); subst.
   cbv [bedrock2_invariant].
-  match goal with H: LowerPipeline.mem_available _ _ _ |- _ => revert H end. generalize m0. eassumption. }
-{ cbv [bedrock2_invariant loop_progress].
+  eapply mem_available_to_seplog. assumption. }
+{ cbv [bedrock2_invariant handle_request_spec].
   intros; eapply MetricWeakestPreconditionProperties.sound_cmd.
   repeat MetricProgramLogic.straightline.
   { eapply MetricSemantics.weaken_call; [eapply link_lightbulb_loop|cbv beta]; try eassumption.
@@ -250,8 +358,6 @@ all :
            MetricLogging.unfold_MetricLog;  MetricLogging.simpl_MetricLog;
                          unfold_MetricLog;                simpl_MetricLog);
           intuition try blia. } }
-
-Unshelve. exact mem_available_to_seplog.
 Qed.
 
 Import OmniSmallstepCombinators.
@@ -260,7 +366,7 @@ Check metric_lightbulb_correct.
 (*
 metric_lightbulb_correct
      : forall (initial : MetricRiscvMachine)
-         (R : map word32 Init.Byte.byte -> Prop),
+         (R : map (Naive.word (2 ^ Nat.log2 32)) Init.Byte.byte -> Prop),
        valid_machine initial ->
        getLog initial = [] ->
        regs_initialized.regs_initialized (getRegs initial) ->
@@ -272,11 +378,11 @@ metric_lightbulb_correct
          (getMem initial) ->
        subset (footpr (program RV32IM (code_start ml) (fst (fst out))))
          (of_list (getXAddrs initial)) ->
-       eventually ToplevelLoop.run1
-         (successively ToplevelLoop.run1
+       eventually riscv.run1
+         (successively riscv.run1
             (fun s s' : MetricRiscvMachine =>
-             loop_progress (getLog s) (getLog s')
-               (getMetrics s' - getMetrics s))) initial
+             handle_request_spec (getLog s) (getLog s') (getMetrics s) (getMetrics s')))
+         initial
  *)
 
 Print Assumptions metric_lightbulb_correct.
@@ -287,9 +393,30 @@ PropExtensionality.propositional_extensionality :
 functional_extensionality_dep :
   forall (A : Type) (B : A -> Type) (f g : forall x : A, B x),
   (forall x : A, f x = g x) -> f = g
+TODO : False
+used in metric_lightbulb_correct to prove
+ successively riscv.run1
+   (fun s s' : MetricRiscvMachine =>
+    exists dt : list Semantics.LogItem,
+      getLog s' = dt ++ getLog s /\
+      (exists ioh : list OP,
+         metric_SPI.mmio_trace_abstraction_relation ioh dt /\
+         ((exists (packet : list Init.Byte.byte) (cmd : bool),
+             (lan9250_recv packet +++ gpio_set 23 cmd) ioh /\
+             lightbulb_packet_rep cmd packet /\
+             (getMetrics s - getMetrics s' <=
+              (60 + 7 * Datatypes.length packet) * mc_spi_xchg_const +
+              lightbulb_handle_cost + Datatypes.length ioh * mc_spi_mul)%metricsL) \/
+          (exists packet : list Init.Byte.byte,
+             lan9250_recv packet ioh /\
+             ~ (exists cmd : bool, lightbulb_packet_rep cmd packet) /\
+             (getMetrics s - getMetrics s' <=
+              (60 + 7 * Datatypes.length packet) * mc_spi_xchg_const +
+              lightbulb_handle_cost + Datatypes.length ioh * mc_spi_mul)%metricsL) \/
+          lan9250_recv_no_packet ioh \/
+          lan9250_recv_packet_too_long ioh \/ (any +++ spi_timeout) ioh))) final
 *)
-
-
+(*------desired code width for papers: max 85 columns------------------------------*)
 (* OLD STUFF BELOW, may be useful for instantiating some assumptions
 
 
